.

EXAMPLE 3.1 Let x1, x2, ln(x) denote x1(x1, x2) = x1(x1, x2) = x2(x1, x2) = x2(x1, x2) = x3(x1, x2) = x3(x1, x2) = x4(x1, x2) = x4(x1, x2) = x5(x1, x2) = x5(x1, x2) = x6(x1, x2) = x6(x1, x2) = x7(x1, x2) = x7(x1, x2) = x8(x1, x2) = x8(x1, x2) = x9(x1, x2) = x9(x1, x2) = x10(x1, x2) = x10(x1, x2) = x11(x1, x2) = x12(x1, x2) = x12(x1, x2) = x13(x1, x2) = x13(x1, x2) = x14(x1, x2) = x14(x1, x2) = x15(x1, x2) = x15(x1, x2) = x16(x1, x2) = x16(x1, x2) = x17(x1, x2) = x17(x1, x2) = x18(x1, x2) = x18(x1, x2) = x19(x1, x2) = x20(x1, x2) = x20(x1, x2) = x21(x1, x2) = x21(x1, x2) = x22(x1, x2) = x22(x1, x2) = x23(x1, x2) = x23(x1, x2) = x24(x1, x2) = x24(x1, x2) = x25(x1, x2) = x25(x1, x2) = x26(x1, x2) = x26(x1, x2) = x27(x1, x2) = x27(x1, x2) = x28(x1, x2) = x28(x1, x2) = x29(x1, x2) = x29(x1, x2) = x30(x1, x2) = x30(x1, x2) = x31(x1, x2) = x31(x1, x2) = x32(x1, x2) = x32(x1, x2) = x33(x1, x2) = x33(x1, x2) = x34(x1, x2) = x34(x1, x2) = x35(x1, x2) = x35(x1, x2) = x36(x1, x2) = x36(x1, x2) = x37(x1, x2) = x37(x1, x2) = x38(x1, x2) = x38(x1, x2) = x39(x1, x2) = x39(x1, x2) = x40(x1, x2) = x40(x1, x2) = x41(x1, x2) = x41(x1, x2) = x42(x1, x2) = x42(x1, x2) = x43(x1, x2) = x43(x1, x2) = x44(x1, x2) = x44(x1, x2) = x45(x1, x2) = x45(x1, x2) = x46(x1, x2) = x46(x1, x2) = x47(x1, x2) = x47(x1, x2) = x48(x1, x2) = x48(x1, x2) = x49(x1, x2) = x49(x1, x2) = x50(x1, x2) = x50(x1, x2) = x51(x1, x2) = x51(x1, x2) = x52(x1, x2) = x52(x1, x2) = x53(x1, x2) = x53(x1, x2) = x54(x1, x2) = x54(x1, x2) = x55(x1, x2) = x55(x1, x2) = x56(x1, x2) = x56(x1, x2) = x57(x1, x2) = x57(x1, x2) = x58(x1, x2) = x58(x1, x2) = x59(x1, x2) = x59(x1, x2) = x60(x1, x2) = x60(x1, x2) = x61(x1, x2) = x61(x1, x2) = x62(x1, x2) = x62(x1, x2) = x63(x1, x2) = x63(x1, x2) = x64(x1, x2) = x64(x1, x2) = x65(x1, x2) = x65(x1, x2) = x66(x1, x2) = x66(x1, x2) = x67(x1, x2) = x67(x1, x2) = x68(x1, x2) = x68(x1, x2) = x69(x1, x2) = x69(x1, x2) = x70(x1, x2) = x70(x1, x2) = x71(x1, x2) = x71(x1, x2) = x72(x1, x2) = x72(x1, x2) = x73(x1, x2) = x73(x1, x2) = x74(x1, x2) = x74(x1, x2) = x75(x1, x2) = x75(x1, x2) = x76(x1, x2) = x76(x1, x2) = x77(x1, x2) = x77(x1, x2) = x78(x1, x2) = x78(x1, x2) = x79(x1, x2) = x79(x1, x2) = x80(x1, x2) = x80(x1, x2